Replenish std/chunk.

theories/std/chunk.v
@@ -1,5 +1,7 @@
 From ml Require Import
   prelude.
+From ml.bi Require Import
+  big_op.
 From ml.language Require Import
   diverge
   notations
@@ -12,7 +14,7 @@ Section heapGS.
 
   Implicit Types i : nat.
   Implicit Types l : loc.
-  Implicit Types v t fn : val.
+  Implicit Types v t fn acc : val.
   Implicit Types vs : list val.
 
   Definition chunk_make : val :=
@@ -20,7 +22,7 @@ Section heapGS.
       if: "sz" < #0 then (
         diverge #()
       ) else if: #0 < "sz" then (
-        AllocN "sz" "v"
+AllocN "sz" "v"
       ) else (
         #(inhabitant : loc)
       ).
@@ -38,6 +40,68 @@ Section heapGS.
       let: "t" := chunk_make "sz" #() in
       chunk_init_aux "t" "sz" "fn" #0 ;;
       "t".
+
+  #[local] Definition chunk_foldli_aux : val :=
+    rec: "chunk_foldli_aux" "t" "sz" "acc" "fn" "i" :=
+      if: "i" = "sz" then (
+        "acc"
+      ) else (
+        "chunk_foldli_aux" "t" "sz" ("fn" "acc" "i" !("t" +ₗ "i")) "fn" ("i" + #1)
+      ).
+  Definition chunk_foldli : val :=
+    λ: "t" "sz" "acc" "fn",
+      chunk_foldli_aux "t" "sz" "acc" "fn" #0.
+  Definition chunk_foldl : val :=
+    λ: "t" "sz" "acc" "fn",
+      chunk_foldli "t" "sz" "acc" (λ: "acc" <> "v", "fn" "acc" "v").
+
+  #[local] Definition chunk_foldri_aux : val :=
+    rec: "chunk_foldri_aux" "t" "fn" "acc" "i" :=
+      if: "i" = #0 then (
+        "acc"
+      ) else (
+        let: "i" := "i" - #1 in
+        "chunk_foldri_aux" "t" "fn" ("fn" "i" !("t" +ₗ "i") "acc") "i"
+      ).
+  Definition chunk_foldri : val :=
+    λ: "t" "sz" "fn" "acc",
+      chunk_foldri_aux "t" "fn" "acc" "sz".
+  Definition chunk_foldr : val :=
+    λ: "t" "sz" "fn" "acc",
+      chunk_foldri "t" "sz" (λ: <> "v" "acc", "fn" "v" "acc") "acc".
+
+  Definition chunk_iteri : val :=
+    λ: "t" "sz" "fn",
+      chunk_foldli "t" "sz" #() (λ: <> "i" "v", "fn" "i" "v" ;; #()).
+  Definition chunk_iter : val :=
+    λ: "t" "sz" "fn",
+      chunk_iteri "t" "sz" (λ: <> "v", "fn" "v").
+
+  Definition chunk_mapi : val :=
+    λ: "t" "sz" "fn",
+      chunk_init "sz" (λ: "i", "fn" "i" !("t" +ₗ "i")).
+  Definition chunk_map : val :=
+    λ: "t" "sz" "fn",
+      chunk_mapi "t" "sz" (λ: <> "v", "fn" "v").
+
+  Definition chunk_copy : val :=
+    λ: "t" "sz" "t'",
+      chunk_iteri "t" "sz" (λ: "i" "v", "t'" +ₗ "i" <- "v").
+
+  Definition chunk_grow : val :=
+    λ: "t" "sz" "sz'" "v",
+      let: "t'" := chunk_make "sz'" "v" in
+      chunk_copy "t" "sz" "t'" ;;
+      "t'".
+  Definition chunk_shrink : val :=
+    λ: "t" "sz" "sz'",
+      let: "t'" := chunk_make "sz'" #() in
+      chunk_copy "t" "sz'" "t'" ;;
+      "t'".
+
+  Definition chunk_clone : val :=
+    λ: "t" "sz",
+      chunk_shrink "t" "sz" "sz".
 
   Section chunk_model.
     Definition chunk_model l dq vs : iProp Σ :=
@@ -677,7 +741,806 @@ Section heapGS.
     rewrite (Z2Nat.id i); last lia. wp_store.
     iSmash.
   Qed.
+
+  #[local] Lemma chunk_foldli_aux_spec i vs_done vs_todo Ψ l dq sz acc fn :
+    i = length vs_done →
+    (sz = i + length vs_todo)%Z →
+    {{{
+      chunk_model (l +ₗ i) dq vs_todo ∗
+      Ψ vs_done acc ∗
+      [∗ list] j ↦ v ∈ vs_todo, ∀ acc,
+        Ψ (vs_done ++ take j vs_todo) acc -∗
+        WP fn acc #(i + j) (v : val) {{ acc', Ψ (vs_done ++ take j vs_todo ++ [v]) acc' }}
+    }}}
+      chunk_foldli_aux #l #sz acc fn #i
+    {{{ acc',
+      RET acc';
+      chunk_model (l +ₗ i) dq vs_todo ∗
+      Ψ (vs_done ++ vs_todo) acc'
+    }}}.
+  Proof.
+    iIntros "%Hi %Hsz %Φ (Hmodel & HΨ & Hfn) HΦ".
+    iInduction vs_todo as [| v vs_todo] "IH" forall (i vs_done Hi Hsz acc); simplify; wp_rec; wp_pures.
+    { rewrite bool_decide_eq_true_2; last (repeat f_equal; lia).
+      wp_pures.
+      iApply "HΦ". iFrame. rewrite right_id //.
+    }
+    iDestruct "Hmodel" as "(H↦ & Hmodel)". rewrite Loc.add_0.
+    iDestruct "Hfn" as "(Hfn & Hfn')". rewrite right_id Z.add_0_r.
+    rewrite bool_decide_eq_false_2; last naive_solver lia.
+    wp_pures. wp_load.
+    wp_bind (fn _ _ _). iApply (wp_wand with "(Hfn [HΨ])"); first by list_simplifier. iIntros "%acc' HΨ".
+    rewrite Z.add_1_r -Nat2Z.inj_succ.
+    wp_apply ("IH" $! _ (vs_done ++ [v]) with "[] [] [Hmodel] HΨ [Hfn']").
+    { rewrite app_length /=. auto with lia. }
+    { auto with lia. }
+    { rewrite /chunk_model.
+      setoid_rewrite Loc.add_assoc.
+      setoid_rewrite <- Nat2Z.inj_add.
+      setoid_rewrite Nat.add_succ_r.
+      iSmash.
+    } {
+      setoid_rewrite <- (assoc (++) vs_done [v]).
+      setoid_rewrite <- Nat2Z.inj_add.
+      setoid_rewrite Nat.add_succ_r.
+      iSmash.
+    }
+    iIntros "%acc'' (Hmodel & HΨ)".
+    iApply "HΦ". rewrite -(assoc (++) vs_done [v]). iFrame.
+    rewrite Loc.add_assoc Z.add_1_r -Nat2Z.inj_succ //.
+  Qed.
+  Lemma chunk_foldli_spec Ψ l dq vs (sz : Z) acc fn :
+    sz = length vs →
+    {{{
+      chunk_model l dq vs ∗
+      Ψ [] acc ∗
+      [∗ list] i ↦ v ∈ vs, ∀ acc,
+        Ψ (take i vs) acc -∗
+        WP fn acc #i (v : val) {{ acc', Ψ (take i vs ++ [v]) acc' }}
+    }}}
+      chunk_foldli #l #sz acc fn
+    {{{ acc',
+      RET acc';
+      chunk_model l dq vs ∗
+      Ψ vs acc'
+    }}}.
+  Proof.
+    iIntros "% %Φ (Hmodel & HΨ & Hfn) HΦ".
+    wp_rec.
+    wp_smart_apply (chunk_foldli_aux_spec 0 [] vs Ψ with "[Hmodel $HΨ $Hfn]"); [done | lia | |].
+    { rewrite Loc.add_0 //. }
+    iIntros "%acc' (Hmodel & HΨ)". rewrite Loc.add_0. iSmash.
+  Qed.
+  Lemma chunk_foldli_spec' Ψ l dq vs (sz : Z) acc fn :
+    sz = length vs →
+    {{{
+      chunk_model l dq vs ∗
+      Ψ [] acc ∗
+      ∀ acc i v,
+      {{{ ⌜vs !! i = Some v⌝ ∗ Ψ (take i vs) acc }}}
+        fn acc #i v
+      {{{ acc', RET acc'; Ψ (take i vs ++ [v]) acc' }}}
+    }}}
+      chunk_foldli #l #sz acc fn
+    {{{ acc',
+      RET acc';
+      chunk_model l dq vs ∗
+      Ψ vs acc'
+    }}}.
+  Proof.
+    iIntros "% %Φ (Hmodel & HΨ & #Hfn) HΦ".
+    wp_apply (chunk_foldli_spec Ψ with "[$Hmodel $HΨ Hfn]"); try done.
+    iApply big_sepL_intro. clear. iIntros "!> %i %v % %acc HΨ".
+    wp_apply ("Hfn" with "[$HΨ //]").
+    iSmash.
+  Qed.
+
+  Lemma chunk_foldl_spec Ψ l dq vs (sz : Z) acc fn :
+    sz = length vs →
+    {{{
+      chunk_model l dq vs ∗
+      Ψ [] acc ∗
+      [∗ list] i ↦ v ∈ vs, ∀ acc,
+        Ψ (take i vs) acc -∗
+        WP fn acc (v : val) {{ acc', Ψ (take i vs ++ [v]) acc' }}
+    }}}
+      chunk_foldl #l #sz acc fn
+    {{{ acc',
+      RET acc';
+      chunk_model l dq vs ∗
+      Ψ vs acc'
+    }}}.
+  Proof.
+    iIntros "% %Φ (Hmodel & HΨ & Hfn) HΦ".
+    wp_rec.
+    wp_smart_apply (chunk_foldli_spec Ψ with "[$Hmodel $HΨ Hfn]"); try done.
+    iApply (big_sepL_mono with "Hfn").
+    iSmash.
+  Qed.
+  Lemma chunk_foldl_spec' Ψ l dq vs (sz : Z) acc fn :
+    sz = length vs →
+    {{{
+      chunk_model l dq vs ∗
+      Ψ [] acc ∗
+      ∀ i v acc,
+      {{{ ⌜vs !! i = Some v⌝ ∗ Ψ (take i vs) acc }}}
+        fn acc v
+      {{{ acc', RET acc'; Ψ (take i vs ++ [v]) acc' }}}
+    }}}
+      chunk_foldl #l #sz acc fn
+    {{{ acc',
+      RET acc';
+      chunk_model l dq vs ∗
+      Ψ vs acc'
+    }}}.
+  Proof.
+    iIntros "% %Φ (Hmodel & HΨ & #Hfn) HΦ".
+    wp_apply (chunk_foldl_spec Ψ with "[$Hmodel $HΨ Hfn]"); try done.
+    iApply big_sepL_intro. clear. iIntros "!> %i %v % %acc HΨ".
+    wp_apply ("Hfn" with "[$HΨ //]").
+    iSmash.
+  Qed.
+
+  #[local] Lemma chunk_foldri_aux_spec i vs_todo vs_done Ψ l dq acc fn :
+    i = length vs_todo →
+    {{{
+      chunk_model l dq vs_todo ∗
+      Ψ acc vs_done ∗
+      [∗ list] j ↦ v ∈ vs_todo, ∀ acc,
+        Ψ acc (drop (S j) vs_todo ++ vs_done) -∗
+        WP fn #j (v : val) acc {{ acc', Ψ acc' (v :: drop (S j) vs_todo ++ vs_done) }}
+    }}}
+      chunk_foldri_aux #l fn acc #i
+    {{{ acc',
+      RET acc';
+      chunk_model l dq vs_todo ∗
+      Ψ acc' (vs_todo ++ vs_done)
+    }}}.
+  Proof.
+    iIntros "%Hi %Φ (Hmodel & HΨ & Hfn) HΦ".
+    iInduction vs_todo as [| v vs_todo] "IH" using rev_ind forall (i vs_done Hi acc); simplify; wp_rec; wp_pures.
+    { iApply ("HΦ" with "[$Hmodel $HΨ]"). }
+    iDestruct "Hmodel" as "(Hmodel & H↦ & _)". iEval (rewrite right_id) in "H↦".
+    iDestruct "Hfn" as "(Hfn' & Hfn & _)".
+    iEval (
+      rewrite
+        right_id
+        -(right_id [] (++) (vs_todo ++ [v])) drop_app_alt /=;
+          last (rewrite app_length /=; lia)
+    ) in "Hfn".
+    rewrite app_length bool_decide_eq_false_2; last naive_solver lia.
+    wp_pures.
+    rewrite Nat.add_1_r Nat2Z.inj_succ Z.sub_1_r Z.pred_succ. wp_load.
+    wp_bind (fn _ _ _). iApply (wp_wand with "(Hfn HΨ)").
+    iIntros "%acc' HΨ".
+    wp_apply ("IH" $! _ (v :: vs_done) with "[//] Hmodel HΨ [Hfn']").
+    { iApply (big_sepL_mono with "Hfn'"). clear. iIntros "%i %w %Hlookup Hfn %acc HΨ".
+      rewrite drop_app_le; last first.
+      { apply lookup_lt_Some in Hlookup. lia. }
+      rewrite -(assoc (++)) /=. iSmash.
+    }
+    iIntros "%acc'' (Hmodel & HΨ)".
+    iApply "HΦ". rewrite -(assoc (++) vs_todo [v]). iFrame. iSplitL; last iSmash.
+    rewrite right_id //.
+  Qed.
+  Lemma chunk_foldri_spec Ψ l dq vs (sz : Z) acc fn :
+    sz = length vs →
+    {{{
+      chunk_model l dq vs ∗
+      Ψ acc [] ∗
+      [∗ list] i ↦ v ∈ vs, ∀ acc,
+        Ψ acc (drop (S i) vs) -∗
+        WP fn #i (v : val) acc {{ acc', Ψ acc' (v :: drop (S i) vs) }}
+    }}}
+      chunk_foldri #l #sz fn acc
+    {{{ acc',
+      RET acc';
+      chunk_model l dq vs ∗
+      Ψ acc' vs
+    }}}.
+  Proof.
+    iIntros "% %Φ (Hmodel & HΨ & Hfn) HΦ".
+    Z_to_nat sz. simplify.
+    wp_rec.
+    wp_smart_apply (chunk_foldri_aux_spec _ vs [] Ψ with "[$Hmodel $HΨ Hfn]"); first done.
+    { iApply (big_sepL_impl with "Hfn").
+      iModIntro. iIntros. rewrite right_id. iSmash.
+    }
+    iIntros "%acc' (Hmodel & HΨ)".
+    iApply "HΦ". iFrame. rewrite right_id //.
+  Qed.
+  Lemma chunk_foldri_spec' Ψ l dq vs (sz : Z) acc fn :
+    sz = length vs →
+    {{{
+      chunk_model l dq vs ∗
+      Ψ acc [] ∗
+      ∀ acc i v,
+      {{{ ⌜vs !! i = Some v⌝ ∗ Ψ acc (drop (S i) vs) }}}
+        fn #i v acc
+      {{{ acc', RET acc'; Ψ acc' (v :: drop (S i) vs) }}}
+    }}}
+      chunk_foldri #l #sz fn acc
+    {{{ acc',
+      RET acc';
+      chunk_model l dq vs ∗
+      Ψ acc' vs
+    }}}.
+  Proof.
+    iIntros "% %Φ (Hmodel & HΨ & #Hfn) HΦ".
+    wp_apply (chunk_foldri_spec Ψ with "[$Hmodel $HΨ Hfn]"); try done.
+    iApply big_sepL_intro. clear. iIntros "!> %i %v % %acc HΨ".
+    wp_apply ("Hfn" with "[$HΨ //]").
+    iSmash.
+  Qed.
+
+  Lemma chunk_foldr_spec Ψ l dq vs (sz : Z) acc fn :
+    sz = length vs →
+    {{{
+      chunk_model l dq vs ∗
+      Ψ acc [] ∗
+      [∗ list] i ↦ v ∈ vs, ∀ acc,
+        Ψ acc (drop (S i) vs) -∗
+        WP fn (v : val) acc {{ acc', Ψ acc' (v :: drop (S i) vs) }}
+    }}}
+      chunk_foldr #l #sz fn acc
+    {{{ acc',
+      RET acc';
+      chunk_model l dq vs ∗
+      Ψ acc' vs
+    }}}.
+  Proof.
+    iIntros "% %Φ (Hmodel & HΨ & Hfn) HΦ".
+    wp_rec.
+    wp_smart_apply (chunk_foldri_spec Ψ with "[$Hmodel $HΨ Hfn]"); try done.
+    iApply (big_sepL_mono with "Hfn").
+    iSmash.
+  Qed.
+  Lemma chunk_foldr_spec' Ψ l dq vs (sz : Z) acc fn :
+    sz = length vs →
+    {{{
+      chunk_model l dq vs ∗
+      Ψ acc [] ∗
+      ∀ i v acc,
+      {{{ ⌜vs !! i = Some v⌝ ∗ Ψ acc (drop (S i) vs) }}}
+        fn v acc
+      {{{ acc', RET acc'; Ψ acc' (v :: drop (S i) vs) }}}
+    }}}
+      chunk_foldr #l #sz fn acc
+    {{{ acc',
+      RET acc';
+      chunk_model l dq vs ∗
+      Ψ acc' vs
+    }}}.
+  Proof.
+    iIntros "% %Φ (Hmodel & HΨ & #Hfn) HΦ".
+    wp_apply (chunk_foldr_spec Ψ with "[$Hmodel $HΨ Hfn]"); try done.
+    iApply big_sepL_intro. clear. iIntros "!> %i %v % %acc HΨ".
+    wp_apply ("Hfn" with "[$HΨ //]").
+    iSmash.
+  Qed.
+
+  Lemma chunk_iteri_spec Ψ l dq vs (sz : Z) fn :
+    sz = length vs →
+    {{{
+      chunk_model l dq vs ∗
+      Ψ [] ∗
+      [∗ list] i ↦ v ∈ vs,
+        Ψ (take i vs) -∗
+        WP fn #i (v : val) {{ _, Ψ (take i vs ++ [v]) }}
+    }}}
+      chunk_iteri #l #sz fn
+    {{{
+      RET #();
+      chunk_model l dq vs ∗
+      Ψ vs
+    }}}.
+  Proof.
+    iIntros "% %Φ (Hmodel & HΨ & Hfn) HΦ".
+    wp_rec.
+    wp_smart_apply (chunk_foldli_spec (λ vs acc, ⌜acc = #()⌝ ∗ Ψ vs)%I with "[$Hmodel $HΨ Hfn]"); try iSmash+.
+    iSplit; first iSmash.
+    iApply (big_sepL_mono with "Hfn"). iIntros "%i %v % Hfn %acc (-> & HΨ)".
+    iSmash.
+  Qed.
+  Lemma chunk_iteri_spec' Ψ l dq vs (sz : Z) fn :
+    sz = length vs →
+    {{{
+      chunk_model l dq vs ∗
+      Ψ [] ∗
+      ∀ i v,
+      {{{ ⌜vs !! i = Some v⌝ ∗ Ψ (take i vs) }}}
+        fn #i v
+      {{{ w, RET w; Ψ (take i vs ++ [v]) }}}
+    }}}
+      chunk_iteri #l #sz fn
+    {{{
+      RET #();
+      chunk_model l dq vs ∗
+      Ψ vs
+    }}}.
+  Proof.
+    iIntros "% %Φ (Hmodel & HΨ & #Hfn) HΦ".
+    wp_apply (chunk_iteri_spec Ψ with "[$Hmodel $HΨ Hfn]"); try done.
+    iApply big_sepL_intro. clear. iIntros "!> %i %v % HΨ".
+    wp_apply ("Hfn" with "[$HΨ //]").
+    iSmash.
+  Qed.
+  Lemma chunk_iteri_spec_disentangled Ψ l dq vs (sz : Z) fn :
+    sz = length vs →
+    {{{
+      chunk_model l dq vs ∗
+      [∗ list] i ↦ v ∈ vs,
+        WP fn #i (v : val) {{ _, Ψ i v }}
+    }}}
+      chunk_iteri #l #sz fn
+    {{{
+      RET #();
+      chunk_model l dq vs ∗
+      [∗ list] i ↦ v ∈ vs, Ψ i v
+    }}}.
+  Proof.
+    iIntros "% %Φ (Hmodel & Hfn) HΦ".
+    set (Ψ' vs := ([∗ list] i ↦ v ∈ vs, Ψ i v)%I).
+    wp_apply (chunk_iteri_spec Ψ' with "[$Hmodel Hfn]"); try done.
+    iSplit; first rewrite /Ψ' //.
+    iApply (big_sepL_mono with "Hfn"). iIntros "%i %v %Hlookup Hfn HΨ'".
+    iApply (wp_wand with "Hfn"). iIntros "%w HΨ". iFrame. iSplitL; last iSmash.
+    rewrite right_id take_length_le //. apply lookup_lt_Some in Hlookup. lia.
+  Qed.
+  Lemma chunk_iteri_spec_disentangled' Ψ l dq vs (sz : Z) fn :
+    sz = length vs →
+    {{{
+      chunk_model l dq vs ∗
+      ∀ i v,
+      {{{ ⌜vs !! i = Some v⌝ }}}
+        fn #i v
+      {{{ w, RET w; Ψ i v }}}
+    }}}
+      chunk_iteri #l #sz fn
+    {{{
+      RET #();
+      chunk_model l dq vs ∗
+      [∗ list] i ↦ v ∈ vs, Ψ i v
+    }}}.
+  Proof.
+    iIntros "% %Φ (Hmodel & #Hfn) HΦ".
+    wp_apply (chunk_iteri_spec_disentangled with "[$Hmodel]"); try done.
+    iApply big_sepL_intro. iIntros "!> %i %v %".
+    iApply ("Hfn" with "[//]").
+    iSmash.
+  Qed.
+
+  Lemma chunk_iter_spec Ψ l dq vs (sz : Z) fn :
+    sz = length vs →
+    {{{
+      chunk_model l dq vs ∗
+      Ψ [] ∗
+      [∗ list] i ↦ v ∈ vs,
+        Ψ (take i vs) -∗
+        WP fn (v : val) {{ _, Ψ (take i vs ++ [v]) }}
+    }}}
+      chunk_iter #l #sz fn
+    {{{
+      RET #();
+      chunk_model l dq vs ∗
+      Ψ vs
+    }}}.
+  Proof.
+    iIntros "% %Φ (Hmodel & HΨ & Hfn) HΦ".
+    wp_rec.
+    wp_smart_apply (chunk_iteri_spec Ψ with "[$Hmodel $HΨ Hfn]"); try done.
+    iApply (big_sepL_mono with "Hfn").
+    iSmash.
+  Qed.
+  Lemma chunk_iter_spec' Ψ l dq vs (sz : Z) fn :
+    sz = length vs →
+    {{{
+      chunk_model l dq vs ∗
+      Ψ [] ∗
+      ∀ i v,
+      {{{ ⌜vs !! i = Some v⌝ ∗ Ψ (take i vs) }}}
+        fn v
+      {{{ w, RET w; Ψ (take i vs ++ [v]) }}}
+    }}}
+      chunk_iter #l #sz fn
+    {{{
+      RET #();
+      chunk_model l dq vs ∗
+      Ψ vs
+    }}}.
+  Proof.
+    iIntros "% %Φ (Hmodel & HΨ & #Hfn) HΦ".
+    wp_apply (chunk_iter_spec Ψ with "[$Hmodel $HΨ Hfn]"); try done.
+    iApply big_sepL_intro. clear. iIntros "!> %i %v % HΨ".
+    wp_apply ("Hfn" with "[$HΨ //]").
+    iSmash.
+  Qed.
+  Lemma chunk_iter_spec_disentangled Ψ l dq vs (sz : Z) fn :
+    sz = length vs →
+    {{{
+      chunk_model l dq vs ∗
+      [∗ list] v ∈ vs,
+        WP fn (v : val) {{ _, Ψ v }}
+    }}}
+      chunk_iter #l #sz fn
+    {{{
+      RET #();
+      chunk_model l dq vs ∗
+      [∗ list] v ∈ vs, Ψ v
+    }}}.
+  Proof.
+    iIntros "% %Φ (Hmodel & Hfn) HΦ".
+    set (Ψ' vs := ([∗ list] v ∈ vs, Ψ v)%I).
+    wp_apply (chunk_iter_spec Ψ' with "[$Hmodel Hfn]"); try done.
+    iSplit; first rewrite /Ψ' //.
+    iApply (big_sepL_mono with "Hfn"). iIntros "%i %v % Hfn HΨ'".
+    iApply (wp_wand with "Hfn"). iIntros "%w HΨ".
+    iFrame. iSmash.
+  Qed.
+  Lemma chunk_iter_spec_disentangled' Ψ l dq vs (sz : Z) fn :
+    sz = length vs →
+    {{{
+      chunk_model l dq vs ∗
+      ∀ v,
+      {{{ ⌜v ∈ vs⌝ }}}
+        fn v
+      {{{ w, RET w; Ψ v }}}
+    }}}
+      chunk_iter #l #sz fn
+    {{{
+      RET #();
+      chunk_model l dq vs ∗
+      [∗ list] v ∈ vs, Ψ v
+    }}}.
+  Proof.
+    iIntros "% %Φ (Hmodel & #Hfn) HΦ".
+    wp_apply (chunk_iter_spec_disentangled with "[$Hmodel]"); try done.
+    iApply big_sepL_intro. iIntros "!> %i %v %".
+    iApply "Hfn"; last iSmash.
+    rewrite elem_of_list_lookup. iSmash.
+  Qed.
+
+  Lemma chunk_mapi_spec Ψ l dq vs (sz : Z) fn :
+    sz = length vs →
+    {{{
+      chunk_model l dq vs ∗
+      Ψ [] [] ∗
+      [∗ list] i ↦ v ∈ vs, ∀ ws,
+        ⌜length ws = i⌝ -∗
+        Ψ (take i vs) ws -∗
+        WP fn #i (v : val) {{ w, Ψ (take i vs ++ [v]) (ws ++ [w]) }}
+    }}}
+      chunk_mapi #l #sz fn
+    {{{ l' ws,
+      RET #l';
+      chunk_model l dq vs ∗
+      chunk_model l' (DfracOwn 1) ws ∗
+      Ψ vs ws ∗
+      if decide (0 < sz)%Z then meta_token l' ⊤ else True
+    }}}.
+  Proof.
+    iIntros "%Hsz %Φ (Hmodel & HΨ & Hfn) HΦ".
+    wp_rec.
+    pose Ψ' ws := (
+      let vs := take (length ws) vs in
+      Ψ vs ws ∗ chunk_model l dq vs
+    )%I.
+    wp_smart_apply (chunk_init_spec Ψ' with "[Hmodel $HΨ Hfn]"); first lia.
+    { iSplit; first rewrite /chunk_model take_0 //.
+      Z_to_nat sz. rewrite Nat2Z.id.
+      iApply (big_sepL_seq_index vs); first naive_solver.
+      iDestruct (big_sepL_sep_2 with "Hmodel Hfn") as "H".
+      iApply (big_sepL_mono with "H"). iIntros "%i %v %Hlookup (H↦ & Hfn) %ws -> (HΨ & Hmodel)".
+      wp_pures. wp_load.
+      iApply (wp_wand with "(Hfn [//] HΨ)"). iIntros "%w HΨ".
+      rewrite /Ψ' app_length /= Nat.add_1_r (take_S_r _ _ v) //.
+      iFrame. iSplitL; last iSmash. rewrite right_id take_length_le //.
+      apply lookup_lt_Some in Hlookup. lia.
+    }
+    iIntros "%l' %ws (%Hws & Hmodel' & (HΨ & Hmodel) & Hmeta)".
+    rewrite Hws Hsz Nat2Z.id firstn_all. iSmash.
+  Qed.
+  Lemma chunk_mapi_spec' Ψ l dq vs (sz : Z) fn :
+    sz = length vs →
+    {{{
+      chunk_model l dq vs ∗
+      Ψ [] [] ∗
+      ∀ i v ws,
+      {{{ ⌜vs !! i = Some v⌝ ∗ Ψ (take i vs) ws }}}
+        fn #i v
+      {{{ w, RET w; Ψ (take i vs ++ [v]) (ws ++ [w]) }}}
+    }}}
+      chunk_mapi #l #sz fn
+    {{{ l' ws,
+      RET #l';
+      chunk_model l dq vs ∗
+      chunk_model l' (DfracOwn 1) ws ∗
+      Ψ vs ws ∗
+      if decide (0 < sz)%Z then meta_token l' ⊤ else True
+    }}}.
+  Proof.
+    iIntros "% %Φ (Hmodel & HΨ & #Hfn) HΦ".
+    wp_apply (chunk_mapi_spec Ψ with "[$Hmodel $HΨ Hfn]"); try done.
+    iApply big_sepL_intro. clear. iIntros "!> %i %v % %ws % HΨ".
+    wp_apply ("Hfn" with "[$HΨ //]").
+    iSmash.
+  Qed.
+  Lemma chunk_mapi_spec_disentangled Ψ l dq vs (sz : Z) fn :
+    sz = length vs →
+    {{{
+      chunk_model l dq vs ∗
+      [∗ list] i ↦ v ∈ vs,
+        WP fn #i (v : val) {{ w, Ψ i v w }}
+    }}}
+      chunk_mapi #l #sz fn
+    {{{ l' ws,
+      RET #l';
+      chunk_model l dq vs ∗
+      chunk_model l' (DfracOwn 1) ws ∗
+      ([∗ list] i ↦ v; w ∈ vs; ws, Ψ i v w) ∗
+      if decide (0 < sz)%Z then meta_token l' ⊤ else True
+    }}}.
+  Proof.
+    iIntros "% %Φ (Hmodel & Hfn) HΦ".
+    set (Ψ' vs ws := ([∗ list] i ↦ v; w ∈ vs; ws, Ψ i v w)%I).
+    wp_apply (chunk_mapi_spec Ψ' with "[$Hmodel Hfn]"); try done.
+    iSplit; first rewrite /Ψ' //.
+    iApply (big_sepL_mono with "Hfn"). iIntros "%i %v %Hlookup Hfn %ws % HΨ'".
+    iApply (wp_wand with "Hfn"). iIntros "%w HΨ". iFrame. iSplitL; last iSmash.
+    rewrite right_id take_length_le //. apply lookup_lt_Some in Hlookup. lia.
+  Qed.
+  Lemma chunk_mapi_spec_disentangled' Ψ l dq vs (sz : Z) fn :
+    sz = length vs →
+    {{{
+      chunk_model l dq vs ∗
+      ∀ i v,
+      {{{ ⌜vs !! i = Some v⌝ }}}
+        fn #i v
+      {{{ w, RET w; Ψ i v w }}}
+    }}}
+      chunk_mapi #l #sz fn
+    {{{ l' ws,
+      RET #l';
+      chunk_model l dq vs ∗
+      chunk_model l' (DfracOwn 1) ws ∗
+      ([∗ list] i ↦ v; w ∈ vs; ws, Ψ i v w) ∗
+      if decide (0 < sz)%Z then meta_token l' ⊤ else True
+    }}}.
+  Proof.
+    iIntros "% %Φ (Hmodel & #Hfn) HΦ".
+    wp_apply (chunk_mapi_spec_disentangled Ψ with "[$Hmodel Hfn]"); try done.
+    iApply big_sepL_intro. clear. iIntros "!> %i %v %".
+    iApply ("Hfn" with "[//]").
+    iSmash.
+  Qed.
+
+  Lemma chunk_map_spec Ψ l dq vs (sz : Z) fn :
+    sz = length vs →
+    {{{
+      chunk_model l dq vs ∗
+      Ψ [] [] ∗
+      [∗ list] i ↦ v ∈ vs, ∀ ws,
+        Ψ (take i vs) ws -∗
+        WP fn (v : val) {{ w, Ψ (take i vs ++ [v]) (ws ++ [w]) }}
+    }}}
+      chunk_map #l #sz fn
+    {{{ l' ws,
+      RET #l';
+      chunk_model l dq vs ∗
+      chunk_model l' (DfracOwn 1) ws ∗
+      Ψ vs ws ∗
+      if decide (0 < sz)%Z then meta_token l' ⊤ else True
+    }}}.
+  Proof.
+    iIntros "% %Φ (Hmodel & HΨ & Hfn) HΦ".
+    wp_rec.
+    wp_smart_apply (chunk_mapi_spec Ψ with "[$Hmodel $HΨ Hfn]"); try done.
+    iApply (big_sepL_mono with "Hfn").
+    iSmash.
+  Qed.
+  Lemma chunk_map_spec' Ψ l dq vs (sz : Z) fn :
+    sz = length vs →
+    {{{
+      chunk_model l dq vs ∗
+      Ψ [] [] ∗
+      ∀ i v ws,
+      {{{ ⌜vs !! i = Some v⌝ ∗ Ψ (take i vs) ws }}}
+        fn v
+      {{{ w, RET w; Ψ (take i vs ++ [v]) (ws ++ [w]) }}}
+    }}}
+      chunk_map #l #sz fn
+    {{{ l' ws,
+      RET #l';
+      chunk_model l dq vs ∗
+      chunk_model l' (DfracOwn 1) ws ∗
+      Ψ vs ws ∗
+      if decide (0 < sz)%Z then meta_token l' ⊤ else True
+    }}}.
+  Proof.
+    iIntros "% %Φ (Hmodel & HΨ & #Hfn) HΦ".
+    wp_apply (chunk_map_spec Ψ with "[$Hmodel $HΨ Hfn]"); try done.
+    iApply big_sepL_intro. clear. iIntros "!> %i %v % %w HΨ".
+    wp_apply ("Hfn" with "[$HΨ //]").
+    iSmash.
+  Qed.
+  Lemma chunk_map_spec_disentangled Ψ l dq vs (sz : Z) fn :
+    sz = length vs →
+    {{{
+      chunk_model l dq vs ∗
+      [∗ list] v ∈ vs,
+        WP fn (v : val) {{ Ψ v }}
+    }}}
+      chunk_map #l #sz fn
+    {{{ l' ws,
+      RET #l';
+      chunk_model l dq vs ∗
+      chunk_model l' (DfracOwn 1) ws ∗
+      ([∗ list] v; w ∈ vs; ws, Ψ v w) ∗
+      if decide (0 < sz)%Z then meta_token l' ⊤ else True
+    }}}.
+  Proof.
+    iIntros "% %Φ (Hmodel & Hfn) HΦ".
+    set (Ψ' vs ws := ([∗ list] v; w ∈ vs; ws, Ψ v w)%I).
+    wp_apply (chunk_map_spec Ψ' with "[$Hmodel Hfn]"); try done.
+    iSplit; first rewrite /Ψ' //.
+    iApply (big_sepL_mono with "Hfn"). iIntros "%i %v % Hfn %ws HΨ'".
+    iApply (wp_wand with "Hfn"). iIntros "%w HΨ".
+    iFrame. iSmash.
+  Qed.
+  Lemma chunk_map_spec_disentangled' Ψ l dq vs (sz : Z) fn :
+    sz = length vs →
+    {{{
+      chunk_model l dq vs ∗
+      ∀ v,
+      {{{ ⌜v ∈ vs⌝ }}}
+        fn v
+      {{{ w, RET w; Ψ v w }}}
+    }}}
+      chunk_map #l #sz fn
+    {{{ l' ws,
+      RET #l';
+      chunk_model l dq vs ∗
+      chunk_model l' (DfracOwn 1) ws ∗
+      ([∗ list] v; w ∈ vs; ws, Ψ v w) ∗
+      if decide (0 < sz)%Z then meta_token l' ⊤ else True
+    }}}.
+  Proof.
+    iIntros "% %Φ (Hmodel & #Hfn) HΦ".
+    wp_apply (chunk_map_spec_disentangled Ψ with "[$Hmodel Hfn]"); try done.
+    iApply big_sepL_intro. clear. iIntros "!> %i %v %".
+    iApply "Hfn"; last iSmash.
+    rewrite elem_of_list_lookup. iSmash.
+  Qed.
+
+  Lemma chunk_copy_spec l dq vs (sz : Z) l' vs' :
+    sz = length vs →
+    sz = length vs' →
+    {{{
+      chunk_model l dq vs ∗
+      chunk_model l' (DfracOwn 1) vs'
+    }}}
+      chunk_copy #l #sz #l'
+    {{{
+      RET #();
+      chunk_model l dq vs ∗
+      chunk_model l' (DfracOwn 1) vs
+    }}}.
+  Proof.
+    iIntros (-> Hsz%(inj _)) "%Φ (Hmodel & Hmodel') HΦ".
+    wp_rec.
+    set (Ψ vs := chunk_model l' (DfracOwn 1) (vs ++ drop (length vs) vs')).
+    wp_smart_apply (chunk_iteri_spec' Ψ with "[$Hmodel Hmodel']"); first done; last first.
+    { iIntros "(Hmodel & HΨ)".
+      iApply "HΦ". iFrame. rewrite /Ψ Hsz drop_all right_id //.
+    }
+    iFrame. clear- Hsz. iIntros "%i %v !> %Φ (%Hlookup & HΨ) HΦ".
+    pose proof Hlookup as Hi%lookup_lt_Some.
+    wp_smart_apply (chunk_set_spec with "HΨ").
+    { rewrite app_length take_length_le; last lia. rewrite drop_length. lia. }
+    iIntros "Hmodel'".
+    iApply "HΦ".
+    rewrite /Ψ Nat2Z.id app_length -assoc Nat.add_1_r insert_app_r_alt take_length_le; [| lia..].
+    rewrite Nat.sub_diag insert_take_drop.
+    - rewrite drop_drop Nat.add_1_r //.
+    - rewrite drop_length. lia.
+  Qed.
+
+  Lemma chunk_grow_spec l dq vs (sz : Z) sz' v :
+    sz = length vs →
+    (sz ≤ sz')%Z →
+    {{{
+      chunk_model l dq vs
+    }}}
+      chunk_grow #l #sz #sz' v
+    {{{ l',
+      RET #l';
+      chunk_model l dq vs ∗
+      chunk_model l' (DfracOwn 1) (vs ++ replicate (Z.to_nat (sz' - sz)) v)
+    }}}.
+  Proof.
+    iIntros "%Hsz %Hsz' %Φ Hmodel HΦ".
+    Z_to_nat sz. Z_to_nat sz'.
+    destruct (Nat.le_exists_sub sz sz') as (dsz & Heq & _); first lia.
+    rewrite (comm Nat.add) in Heq. subst sz'.
+    wp_rec.
+    wp_smart_apply (chunk_make_spec with "[//]"); first lia. iIntros "%l' (Hmodel' & _)".
+    rewrite Nat2Z.id replicate_add.
+    iDestruct (chunk_model_app_2 with "Hmodel'") as "(Hmodel'1 & Hmodel'2)"; first done.
+    wp_smart_apply (chunk_copy_spec with "[$Hmodel $Hmodel'1]"); first done.
+    { rewrite replicate_length. lia. }
+    iIntros "(Hmodel & Hmodel'1)".
+    rewrite -Nat2Z.inj_sub; last lia. rewrite Nat2Z.id Nat.sub_add' replicate_length Hsz.
+    iDestruct (chunk_model_app_1 with "Hmodel'1 Hmodel'2") as "Hmodel'"; first done.
+    iSmash.
+  Qed.
+
+  Lemma chunk_shrink_spec l dq vs (sz : Z) sz' :
+    sz = length vs →
+    (0 ≤ sz' ≤ sz)%Z →
+    {{{
+      chunk_model l dq vs
+    }}}
+      chunk_shrink #l #sz #sz'
+    {{{ l',
+      RET #l';
+      chunk_model l dq vs ∗
+      chunk_model l' (DfracOwn 1) (take (Z.to_nat sz') vs)
+    }}}.
+  Proof.
+    iIntros "%Hsz %Hsz' %Φ Hmodel HΦ".
+    Z_to_nat sz. Z_to_nat sz'.
+    destruct (Nat.le_exists_sub sz' sz) as (dsz & Heq & _); first lia.
+    rewrite (comm Nat.add) in Heq. subst sz.
+    wp_rec.
+    wp_smart_apply (chunk_make_spec with "[//]"); first lia. iIntros "%l' (Hmodel' & _)".
+    rewrite Nat2Z.id -{1}(take_drop sz' vs).
+    iDestruct (chunk_model_app_2 with "Hmodel") as "(Hmodel1 & Hmodel2)"; first done.
+    wp_smart_apply (chunk_copy_spec with "[$Hmodel1 $Hmodel']").
+    { rewrite take_length_le; lia. }
+    { rewrite replicate_length. lia. }
+    iIntros "(Hmodel1 & Hmodel')".
+    rewrite take_length_le; last lia.
+    iDestruct (chunk_model_app_1 with "Hmodel1 Hmodel2") as "Hmodel".
+    { rewrite take_length_le; lia. }
+    rewrite take_drop.
+    iSmash.
+  Qed.
+
+  Lemma chunk_clone_spec l dq vs (sz : Z) :
+    sz = length vs →
+    {{{
+      chunk_model l dq vs
+    }}}
+      chunk_clone #l #sz
+    {{{ l',
+      RET #l';
+      chunk_model l dq vs ∗
+      chunk_model l' (DfracOwn 1) vs
+    }}}.
+  Proof.
+    iIntros "%Hsz %Φ Hmodel HΦ".
+    wp_rec.
+    wp_smart_apply (chunk_shrink_spec with "Hmodel"); [lia.. |].
+    iIntros "%l' (Hmodel & Hmodel')".
+    iApply "HΦ".
+    rewrite Hsz Nat2Z.id firstn_all. iSmash.
+  Qed.
 End heapGS.
 
 #[global] Opaque chunk_make.
 #[global] Opaque chunk_init.
+#[global] Opaque chunk_foldli.
+#[global] Opaque chunk_foldl.
+#[global] Opaque chunk_foldri.
+#[global] Opaque chunk_foldr.
+#[global] Opaque chunk_iteri.
+#[global] Opaque chunk_iter.
+#[global] Opaque chunk_mapi.
+#[global] Opaque chunk_map.
+#[global] Opaque chunk_copy.
+#[global] Opaque chunk_grow.
+#[global] Opaque chunk_shrink.
+#[global] Opaque chunk_clone.
+
+#[global] Opaque chunk_model.
+#[global] Opaque chunk_span.
